Make samplers and `While` loops `opaque` (#100)
Reason: For while loops, the definition is not very helpful, it's better
to rely on lemmas around it for proofs. When calling samplers, we should
also not rely on their internals, but on their correctness properties.
It also reduces resource usage.

As a concession, this PR also adds a postcondition for `While` to avoid
having to call a lemma to handle the case of a while loop immediately
exiting.

By submitting this pull request, I confirm that my contribution is made
under the terms of the [MIT
license](https://github.com/dafny-lang/dafny/blob/master/LICENSE.txt).

src/ProbabilisticProgramming/Loops.dfy
@@ -36,8 +36,12 @@ module Loops {
     forall init :: Quantifier.AlmostSurely(p(init))
   }
 
+  // Definition of while loops.
+  // This definition is opaque because the details are not very useful.
+  // For proofs, use the lemma `WhileUnroll`.
   // Equation (3.25)
-  ghost function While<A>(condition: A -> bool, body: A -> Monad.Hurd<A>, init: A): (f: Monad.Hurd<A>)
+  opaque ghost function While<A>(condition: A -> bool, body: A -> Monad.Hurd<A>, init: A): (f: Monad.Hurd<A>)
+    ensures forall s: Rand.Bitstream :: !condition(init) ==> f(s) == Monad.Return(init)(s)
   {
     (s: Rand.Bitstream) =>
       if WhileCutTerminates(condition, body, init, s)
@@ -77,6 +81,8 @@ module Loops {
     WhileTerminatesAlmostSurely(reject, body)
   }
 
+  // Definition of until loops (rejection sampling).
+  // For proofs, use the lemma `UntilUnroll`.
   // Definition 44
   ghost function Until<A>(proposal: Monad.Hurd<A>, accept: A -> bool): (f: Monad.Hurd<A>)
     requires UntilTerminatesAlmostSurely(proposal, accept)
@@ -179,9 +185,11 @@ module Loops {
     assert loop == unrolled by {
       calc {
         loop;
+        { reveal While(); }
         WhileCut(condition, body, init, fuel)(s);
         { WhileCutUnroll(condition, body, init, s, init', s', fuel'); }
         WhileCut(condition, body, init', fuel')(s');
+        { reveal While(); }
         unrolled;
       }
     }
@@ -324,9 +332,10 @@ module Loops {
   {
     var reject := (a: A) => !accept(a);
     var body := (a: A) => proposal;
-    forall init: A {
+    var f := (init: A) => While(reject, body, init);
+    forall init: A ensures Independence.IsIndep(f(init)) {
       WhileIsIndep(reject, body, init);
     }
-    Independence.BindIsIndep(proposal, (init: A) => While(reject, body, init));
+    Independence.BindIsIndep(proposal, f);
   }
 }
